monadic.dfy
@@ -1,89 +1,13 @@
 include "std.dfy"
 include "util.dfy"
 include "lang.dfy"
+include "evaluator.dfy"
 
 import opened def.std
 import opened util
 import opened lang
+import opened evaluator
 
-function eval(env : Env, e : Term) : Option<Val>
-    decreases e , 0
-{
-  match e {
-    case Var(x) => lookup(env,x)
-    case Lit(v) => Some(v)
-    case Add(e1,e2) => 
-        var n1 :- evalInt(env,e1);
-        var n2 :- evalInt(env,e2);
-        Some(IntVal(n1 + n2))
-    case Sub(e1,e2) => 
-        var n1 :- evalInt(env,e1);
-        var n2 :- evalInt(env,e2);
-        Some(IntVal(n1 - n2))
-    case Or(e1,e2) =>
-        var b1 :- evalBool(env,e1);
-        var b2 :- evalBool(env,e2);
-        Some(BoolVal(b1 || b2))
-    case And(e1,e2) =>
-        var b1 :- evalBool(env,e1);
-        var b2 :- evalBool(env,e2);
-        Some(BoolVal(b1 && b2))
-    case Eq(e1,e2) =>
-        var v1 :- eval(env,e1);
-        var v2 :- eval(env,e2);
-        Some(BoolVal(v1 == v2))
-    case Record(em) =>
-        var m :- evalRecordExpr(env,em);
-        Some(RecordVal(m))
-    case RecordProj(e',f) => 
-        var m :- evalRecord(env,e');
-        lookup(m,f)
-    case If(eb,e1,e2) =>
-        var b :- evalBool(env,eb);
-        if b then eval(env,e1) else eval(env,e2)
-  }
-}
-
-function evalInt(env : Env, e : Term) : Option<int>
-    decreases e , 1
-{
-    var v :- eval(env,e);
-    match v {
-        case IntVal(n) => Some(n)
-        case _ => None
-    }
-}
-
-function evalBool(env : Env, e : Term) : Option<bool>
-    decreases e , 1
-{
-    var v :- eval(env,e);
-    match v {
-        case BoolVal(b) => Some(b)
-        case _ => None
-    }
-}
-
-function evalRecord(env : Env, e : Term) : Option<map<string,Val>>
-    decreases e , 1
-{
-    var v :- eval(env,e);
-    match v {
-        case RecordVal(m) => Some(m)
-        case _ => None
-    }
-}
-
-function evalRecordExpr(env : Env, es : seq<(string,Term)>) : Option<map<string,Val>>
-    decreases es
-{
-  if es == [] then Some(map[])
-  else
-    var k := es[0].0;
-    var v :- eval(env,es[0].1);
-    var vm :- evalRecordExpr(env,es[1..]);
-    if k in vm.Keys then Some(vm) else Some(vm[k := v])
-}
 
 function infer(ctx : Ctx, e : Term) : Option<Ty>
     decreases e, 0
